LeanGrow/Src/Data/CTrie/Proofs/Membership.lean
@@ -1,0 +1,215 @@
+
+
+/-
+Copyright (c) 2026 Yves Jäckle. All rights reserved.
+Released under Apache 2.0 license as described in the file LICENSE.
+Author: Yves Jäckle.
+-/
+
+
+import LeanGrow.Src.Utils.Std.ByteArray
+import LeanGrow.Src.Utils.Std.Array
+import LeanGrow.Src.Data.Amalgames
+
+import Lean.Meta.Basic
+
+open Lean
+
+
+
+inductive CTrie (α : Type _) where
+  | leaf : CTrie α
+  | fruit : α → CTrie α
+  | lnode1 : ByteArray → CTrie α → CTrie α
+  | fnode1 : α → ByteArray → CTrie α → CTrie α
+  | lnode : Array ByteArray → Array (CTrie α) → CTrie α
+  | fnode : α → Array ByteArray → Array (CTrie α) → CTrie α
+deriving Inhabited, Repr, BEq
+
+
+namespace CTrie
+
+variable {α : Sort _}
+
+set_option autoImplicit true
+
+
+-- # Exmpty and inhabited
+
+def empty : CTrie α := leaf
+
+instance : EmptyCollection (CTrie α) :=
+  ⟨empty⟩
+
+instance : Inhabited (CTrie α) where
+  default := empty
+
+
+inductive CTrieZipU (α : Type _) where
+  | nil : CTrieZipU α
+  | leaf : CTrieZipU α → CTrieZipU α
+  | fruit : α → CTrieZipU α → CTrieZipU α
+  | lnode1 : ByteArray → CTrieZipU α → CTrieZipU α
+  | fnode1 : α → ByteArray → CTrieZipU α → CTrieZipU α
+  | lnode : Array ByteArray → Array (CTrie α) → Nat → CTrieZipU α → CTrieZipU α
+  | fnode : α → Array ByteArray → Array (CTrie α) → Nat → CTrieZipU α → CTrieZipU α
+deriving Inhabited, Repr, BEq
+
+
+
+partial def unzip (z : CTrieZipU α) : CTrie α → CTrieZipU α
+  | .leaf => .leaf z
+  | .fruit v => .fruit v z
+  | .lnode1 c t => unzip (.lnode1 c z) t
+  | .fnode1 v c t => unzip (.fnode1 v c z) t
+  | .lnode cs ts => unzip (.lnode cs ts 0 z) ts[0]!
+  | .fnode v cs ts => unzip (.fnode v cs ts 0 z) ts[0]!
+
+
+partial def cleanUp (t : CTrie α) : CTrieZipU α → CTrie α
+  | .nil => t
+  | .leaf nx => cleanUp (.leaf) nx
+  | .fruit v nx => cleanUp (.fruit v) nx
+  | .lnode1 c nx =>
+      match t with
+      | .leaf => cleanUp t nx
+      | .lnode1 c' k => cleanUp (.lnode1 (c ++ c') k) nx
+      | _ =>
+        if c.isEmpty
+        then cleanUp t nx
+        else cleanUp (.lnode1 c t) nx
+  | .fnode1 v c nx =>
+      match t with
+      | .leaf => cleanUp (.fruit v) nx
+      | .lnode1 c' k => cleanUp (.fnode1 v (c ++ c') k) nx
+      | _ => cleanUp (.fnode1 v c t) nx
+  | .lnode cs ts idx nx =>
+      if idx == ts.size - 1
+      then
+        let ts := ts.set! idx t
+        let (nax,ncx) := clean_inner cs ts [] [] cs.size
+        match nax, ncx with
+        | [], _ => cleanUp (.leaf) nx
+        | [NAX], [NCX] => cleanUp (.lnode1 NAX NCX) nx
+        | _, _ => cleanUp (.lnode nax.toArray ncx.toArray) nx
+      else
+        let ts := ts.set! idx t
+        let NX := unzip (.lnode cs ts (idx+1) nx) ts[idx+1]!
+        cleanUp t NX
+  | .fnode v cs ts idx nx =>
+      if idx == ts.size - 1
+      then
+        let ts := ts.set! idx t
+        let (nax,ncx) := clean_inner cs ts [] [] cs.size
+        match nax, ncx with
+        | [], _ => cleanUp (.fruit v) nx
+        | [NAX], [NCX] => cleanUp (.fnode1 v NAX NCX) nx
+        | _, _ => cleanUp (.fnode v nax.toArray ncx.toArray) nx
+      else
+        let ts := ts.set! idx t
+        let NX := unzip (.fnode v cs ts (idx+1) nx) ts[idx+1]!
+        cleanUp t NX
+where
+  clean_inner (cs : Array ByteArray) (ts : Array (CTrie α)) (bs : List ByteArray) (Ts : List (CTrie α)) : Nat → List ByteArray × List (CTrie α)
+    | 0 => (bs,Ts)
+    | n+1 =>
+        let X := ts[n]!
+        match X with
+        | .leaf => clean_inner cs ts bs Ts n
+        | _ => clean_inner cs ts ((cs[n]!) :: bs) (X :: Ts) n
+
+@[inline]
+def clean (t : CTrie α) : CTrie α :=
+  cleanUp t (unzip .nil t)
+
+
+-- # Find, toList
+
+private inductive upsert_help_type where
+  | hit (pos : Nat) (len : Nat)
+  | ins (pos : Nat)
+deriving Inhabited, BEq, Repr
+
+@[inline]
+private def upsert_help (cs : Array ByteArray) (i : Nat) (s : ByteArray) (si : UInt8) : upsert_help_type :=
+  let rec go : Nat → upsert_help_type
+    | 0 => .ins 0
+    | n+1 =>
+        let c := (cs[n]!)
+        let j := ByteArray.getLongestMatch_wOffset i s c
+        if j == 0
+        then
+          if si < c.get! 0
+          then go n
+          else .ins (n+1)
+        else .hit n j
+  go cs.size
+
+
+def find?.go (s : ByteArray) (i : Nat) : CTrie α → Option α
+    | .leaf => .none
+    | .fruit v => v
+    | .lnode1 c t =>
+          if i = s.size
+          then .none
+          else
+            let j := ByteArray.getLongestMatch_wOffset i s c
+            if j == c.size
+            then find?.go s (i+j) t
+            else .none
+    | .fnode1 v c t =>
+          if i = s.size
+          then v
+          else
+            let j := ByteArray.getLongestMatch_wOffset i s c
+            if j == c.size
+            then find?.go s (i+j) t
+            else .none
+    | .lnode cs ts =>
+          if i = s.size
+          then .none
+          else
+            match CTrie.upsert_help cs i s (s.get! i) with
+            | .ins _ => .none
+            | .hit idx len =>
+                  if len == (cs[idx]!).size
+                  then find?.go s (i+len) (ts[idx]!)
+                  else .none
+    | .fnode v cs ts =>
+          if i = s.size
+          then v
+          else
+            match CTrie.upsert_help cs i s (s.get! i) with
+            | .ins _ => .none
+            | .hit idx len =>
+                  if len == (cs[idx]!).size
+                  then find?.go s (i+len) (ts[idx]!)
+                  else .none
+termination_by _ => s.size - i
+decreasing_by
+  · sorry
+  · sorry
+  · sorry -- requires that CTries have nonempty discri bytearrays at nodes ...
+  · sorry
+
+
+
+
+def find? (t : CTrie α) (s : ByteArray) : Option α :=
+  find?.go s 0 t
+
+
+example (t : CTrie α) (s : ByteArray) {a}
+  (h : t.find? s = .some a)
+  : t.clean.find? s = .some a := by
+    revert h
+    apply @CTrie.rec _
+      (fun t => t.find? s = .some a → t.clean.find? s = .some a)
+      (fun _ => True) (fun _ => True)
+    · intro h
+      dsimp [CTrie.find?] at h
+      unfold CTrie.find?.go at h
+      contradiction
+    all_goals sorry
+
+#check CTrie.find?.go.eq_1
